Filesys/PathBasedFSRefinement.i.dfy
@@ -1,7 +1,6 @@
 // Copyright 2018-2021 VMware, Inc., Microsoft Inc., Carnegie Mellon University, ETH Zurich, and University of Washington
 // SPDX-License-Identifier: BSD-2-Clause
 
-// include "FileSystem.s.dfy"
 include "FileSystemInv.i.dfy"
 include "PathBasedFSInv.i.dfy"
 include "../lib/Base/Maps.i.dfy"
@@ -22,7 +21,7 @@ module PathBasedFSRefinement {
   function {:opaque} IPathMap(fs: P.FileSys) : (path_map: F.PathMap)
   requires PInv.Inv(fs)
   ensures F.PathMapComplete(path_map)
-  ensures forall p :: path_map[p] == if P.PathExists(fs, p) then P.GetMeta(fs, p).id else Nonexistent
+  // ensures forall p :: path_map[p] == if P.PathExists(fs, p) then P.GetMeta(fs, p).id else Nonexistent
   {
     imap path :: if P.PathExists(fs, path) then P.GetMeta(fs, path).id else Nonexistent
   }
@@ -30,10 +29,11 @@ module PathBasedFSRefinement {
   function {:opaque} IMetaMap(fs: P.FileSys) : (meta_map: F.MetaView)
   requires PInv.Inv(fs)
   ensures forall id :: id in meta_map
-  ensures forall id | id !in IPathMap(fs).Values :: meta_map[id] == EmptyMeta
-  ensures forall p :: meta_map[IPathMap(fs)[p]] == P.GetMeta(fs, p)
+  // ensures forall id | id !in IPathMap(fs).Values :: meta_map[id] == EmptyMeta
+  // ensures forall p :: meta_map[IPathMap(fs)[p]] == P.GetMeta(fs, p)
   {
     var path_map := IPathMap(fs);
+    reveal_IPathMap();
 
     imap id : ID :: 
       if id in path_map.Values
@@ -44,10 +44,11 @@ module PathBasedFSRefinement {
   function {:opaque} IDataMap(fs: P.FileSys) : (data_map: F.DataView)
   requires PInv.Inv(fs)
   ensures forall id :: id in data_map
-  ensures forall id | id !in IPathMap(fs).Values :: data_map[id] == EmptyData()
-  ensures forall p :: data_map[IPathMap(fs)[p]] == P.GetData(fs, p)
+  // ensures forall id | id !in IPathMap(fs).Values :: data_map[id] == EmptyData()
+  // ensures forall p :: data_map[IPathMap(fs)[p]] == P.GetData(fs, p)
   {
     var path_map := IPathMap(fs);
+    reveal_IPathMap();
 
     imap id : ID :: 
       if id in path_map.Values
@@ -74,18 +75,40 @@ module PathBasedFSRefinement {
     }
   }
 
-  function I(fs: P.FileSys) : (F.FileSys)
+  function I(fs: P.FileSys) : (i_fs: F.FileSys)
   requires PInv.Inv(fs)
+  ensures F.WF(i_fs)
+  ensures FInv.Inv(i_fs)
   {
-    F.FileSys(IPathMap(fs), IMetaMap(fs), IDataMap(fs))
+    var i_fs := F.FileSys(IPathMap(fs), IMetaMap(fs), IDataMap(fs));
+    assert FInv.Inv(i_fs) by { reveal_IPathMap(); reveal_IMetaMap(); reveal_IDataMap(); }
+    i_fs
   }
 
   /// Refinement Proofs
 
-  lemma InvImpliesInv(fs: P.FileSys)
+  // TODO: comment out
+  // lemma InvImpliesInv(fs: P.FileSys)
+  // requires PInv.Inv(fs)
+  // ensures FInv.Inv(I(fs))
+  // {
+  // }
+
+  lemma GetMetaEquiv(fs: P.FileSys, path: Path)
   requires PInv.Inv(fs)
-  ensures FInv.Inv(I(fs))
+  ensures P.GetMeta(fs, path) == I(fs).meta_map[I(fs).path_map[path]]
   {
+    reveal_IPathMap();
+    reveal_IMetaMap();
+  }
+
+  lemma GetDataEquiv(fs: P.FileSys, path: Path)
+  requires PInv.Inv(fs)
+  ensures P.GetData(fs, path) == I(fs).data_map[I(fs).path_map[path]]
+  {
+    reveal_IPathMap();
+    reveal_IMetaMap();
+    reveal_IDataMap();
   }
 
   lemma NoAliasEquiv(fs: P.FileSys, path: Path)
@@ -93,13 +116,20 @@ module PathBasedFSRefinement {
   requires P.PathExists(fs, path)
   ensures P.NoAlias(fs, path) == F.NoAlias(I(fs), path)
   {
+    reveal_IPathMap();
   }
+
+  // lemma PathExists
 
   lemma RefinesInit(fs: P.FileSys)
   requires P.Init(fs)
   requires PInv.Inv(fs)
   ensures F.Init(I(fs))
   {
+    reveal_IPathMap();
+    reveal_IMetaMap();
+    reveal_IDataMap();
+
     assert I(fs).path_map[RootDir] == RootID; // observe
   }
 
@@ -149,6 +179,7 @@ module PathBasedFSRefinement {
   requires P.GetAttr(fs, fs', path, attr)
   ensures F.GetAttr(I(fs), I(fs'), path, attr)
   {
+    GetMetaEquiv(fs, path);
   }
 
   lemma RefinesReadLink(fs: P.FileSys, fs': P.FileSys, path: Path, link_path: Path)
@@ -156,8 +187,10 @@ module PathBasedFSRefinement {
   requires P.ReadLink(fs, fs', path, link_path)
   ensures F.ReadLink(I(fs), I(fs'), path, link_path)
   {
+    GetMetaEquiv(fs, path);
   }
 
+  // maybe before fixing all of these proof we should check if rename does work like this.
   lemma RefinesCreate(fs: P.FileSys, fs': P.FileSys, path: Path, m: MetaData)
   requires PInv.Inv(fs)
   requires PInv.Inv(fs')
@@ -170,17 +203,26 @@ module PathBasedFSRefinement {
     var parent_id := P.GetMeta(fs, parent_dir).id;
     var parent_m' := P.UpdatePathTime(fs.content, parent_dir, m.mtime);
 
+    reveal_IPathMap();
+
     assert !P.PathExists(fs, path);
+    assert i_fs'.path_map == i_fs.path_map[path := m.id];
+
+    reveal_IMetaMap();
+    reveal_IDataMap();
+
     assert i_fs.meta_map[m.id].EmptyMeta?;
     assert i_fs.data_map[m.id] == P.GetData(fs, path) == EmptyData();
-    assert i_fs'.path_map == i_fs.path_map[path := m.id];
 
     forall id 
     ensures i_fs'.meta_map[id] == i_fs.meta_map[m.id := m][parent_id := parent_m'][id]
     ensures i_fs'.data_map[id] == i_fs.data_map[id]
     {
+
       if id in i_fs.path_map.Values {
         if id == parent_id {
+                  assume false;
+
           calc {
             i_fs.meta_map[m.id := m][parent_id := parent_m'][id];
             P.GetMeta(fs', parent_dir);
@@ -193,7 +235,10 @@ module PathBasedFSRefinement {
             i_fs.data_map[parent_id];
           }
         } else {
+
           if exists p :: P.PathExists(fs, p) && P.GetMeta(fs, p).id == id {
+                              assume false;
+
             var p :| P.PathExists(fs, p) && P.GetMeta(fs, p).id == id;
             calc {
               i_fs.meta_map[id];
@@ -208,13 +253,14 @@ module PathBasedFSRefinement {
               P.GetData(fs, p);
               i_fs.data_map[id];
             }
-          } else {
-            assert id.Nonexistent?;
-            InvImpliesInv(fs);
-            InvImpliesInv(fs');
           }
+          
+          // else {
+          //   assert id.Nonexistent?;
+          // }
         }
       } else {
+        assume false;
         if id == m.id {
           calc {
             i_fs'.meta_map[id];
@@ -272,8 +318,8 @@ module PathBasedFSRefinement {
     ensures i_fs'.data_map[id] == i_fs.data_map[path_id := F.DataDelete(i_fs, path)][id]
     {
       if id == Nonexistent {
-        InvImpliesInv(fs);
-        InvImpliesInv(fs');
+        // InvImpliesInv(fs);
+        // InvImpliesInv(fs');
       } else if id in i_fs.path_map.Values {
         if id == parent_id {
           assert i_fs.path_map[parent_dir] == i_fs'.path_map[parent_dir];
@@ -323,13 +369,277 @@ module PathBasedFSRefinement {
     assert F.Delete(i_fs, i_fs', path, ctime);
   }
 
-  lemma RefinesRename(fs: P.FileSys, fs': P.FileSys, source: Path, dest: Path, ctime: Time)
+  lemma RefinesRenamePathMap(fs: P.FileSys, fs': P.FileSys, src: Path, dst: Path, ctime: Time)
   requires PInv.Inv(fs)
   requires PInv.Inv(fs')
-  requires P.Rename(fs, fs', source, dest, ctime)
-  ensures F.Rename(I(fs), I(fs'), source, dest, ctime)
+  requires P.Rename(fs, fs', src, dst, ctime)
+  requires dst != RootDir
+  ensures I(fs').path_map == F.PathMapRename(I(fs), src, dst)
   {
-    assume false;
+    var i_fs := I(fs);
+    var i_fs' := I(fs');
+
+    var src_m := P.GetMeta(fs, src);
+    var src_id := P.GetMeta(fs, src).id;
+    var dst_m := P.GetMeta(fs, dst);
+
+    forall path
+    ensures i_fs'.path_map[path] == F.PathMapRename(i_fs, src, dst)[path]
+    {
+      reveal_IPathMap();
+      if path == dst {
+        assert src + path[|dst|..] == src;
+        assert i_fs.path_map[src] == src_id;
+        assert i_fs'.path_map[path] == src_id;
+        assert F.PathMapRename(i_fs, src, dst)[dst] == i_fs.path_map[src];
+      } else if BeneathDir(dst, path) {
+        var srcpath := src + path[|dst|..];
+        assert fs'.content.meta_map[path] == fs.content.meta_map[srcpath];
+      } else if path == src || BeneathDir(src, path) {
+        assert P.GetMeta(fs', path) == EmptyMeta;
+        assert i_fs'.path_map[path] == Nonexistent; 
+      } else if path == GetParentDir(src) || path == GetParentDir(dst) {
+        assert fs'.content.meta_map[path] == P.UpdatePathTime(fs.content, path, ctime);
+        assert fs'.content.meta_map[path].id == fs.content.meta_map[path].id;
+      }
+    }
+    Maps.IMapEquivalent(i_fs'.path_map, F.PathMapRename(i_fs, src, dst));
+  }
+
+  lemma meow(fs: P.FileSys, fs': P.FileSys, src: Path, dst: Path, ctime: Time)
+  requires PInv.Inv(fs)
+  requires PInv.Inv(fs')
+  requires P.Rename(fs, fs', src, dst, ctime)
+  requires dst != RootDir
+  requires P.PathExists(fs, dst)
+  requires I(fs').path_map == F.PathMapRename(I(fs), src, dst)
+  ensures I(fs').meta_map[P.GetMeta(fs, dst).id] == F.MetaMapRename(I(fs), src, dst, ctime)[P.GetMeta(fs, dst).id]
+  ensures I(fs').data_map[P.GetMeta(fs, dst).id] == I(fs).data_map[P.GetMeta(fs, dst).id := F.DataDelete(I(fs), dst)][P.GetMeta(fs, dst).id]
+  {
+    var i_fs := I(fs);
+    var i_fs' := I(fs');
+
+    var dst_id := P.GetMeta(fs, dst).id;
+    assert dst_id == i_fs.path_map[dst] by { reveal_IPathMap(); }
+
+    var src_id := P.GetMeta(fs, src).id;
+    assert src_id == i_fs.path_map[src] by { reveal_IPathMap(); }
+
+    var src_parent_dir := GetParentDir(src);
+    var src_parent_id := P.GetMeta(fs, src_parent_dir).id;
+    assert src_parent_id == i_fs.path_map[src_parent_dir] by { reveal_IPathMap(); }
+
+    var dst_parent_dir := GetParentDir(dst);
+    var dst_parent_id := P.GetMeta(fs, dst_parent_dir).id;
+    assert dst_parent_id == i_fs.path_map[dst_parent_dir] by { reveal_IPathMap(); }
+
+    assert dst_id != src_id;
+    assert dst_id != src_parent_id;
+    assert dst_id != dst_parent_id;
+
+    NoAliasEquiv(fs, dst);
+    if P.NoAlias(fs, dst) {
+      assert dst_id !in i_fs'.path_map.Values; // observe
+      assert i_fs'.meta_map[dst_id] == EmptyMeta by { reveal_IMetaMap(); }
+      assert i_fs'.data_map[dst_id] == EmptyData() by { reveal_IDataMap(); }
+    } else {
+      assert exists p :: P.PathExists(fs, p) && P.GetMeta(fs, p).id == dst_id by { reveal_IPathMap(); }
+      var p :| P.PathExists(fs, p) && P.GetMeta(fs, p).id == dst_id && p != dst;
+      assert i_fs.path_map[p] == dst_id by { reveal_IPathMap(); }
+
+      GetMetaEquiv(fs, dst);
+      assert F.MetaMapRename(i_fs, src, dst, ctime)[dst_id] == F.MetaDataDelete(i_fs, dst, ctime);
+      assert F.MetaMapRename(i_fs, src, dst, ctime)[dst_id] == F.MetaDataUpdateCTime(i_fs.meta_map[dst_id], ctime);
+
+      var dst_m := fs.content.meta_map[dst];
+      assert dst_m.RedirectMeta?;
+      assert fs.content.meta_map[p] == dst_m;
+      
+      assert p != dst;
+      assert p != src;
+      assert !BeneathDir(dst, p) by {
+        if BeneathDir(dst, p) {
+          PInv.NoValidBeneathDir(fs, dst, p);
+        }
+      }
+
+      if BeneathDir(src, p) {
+        var dstpath := dst + p[|src|..];
+        assert p == src + dstpath[|dst|..];
+        assert i_fs'.path_map[dstpath] == i_fs.path_map[p];
+        assert i_fs'.path_map[dstpath] == dst_id;
+        GetMetaEquiv(fs, p);
+        GetMetaEquiv(fs', dstpath);
+        GetDataEquiv(fs, p);
+        GetDataEquiv(fs', dstpath);
+      } else {
+        assert i_fs'.path_map[p] == dst_id;
+        assert fs'.content.meta_map[p] == dst_m;
+        GetMetaEquiv(fs', p);
+        GetDataEquiv(fs, p);
+        GetDataEquiv(fs', p);
+      }
+    }
+  }
+
+  lemma {:timeLimitMultiplier 2} RefinesRenameMetaMap(fs: P.FileSys, fs': P.FileSys, src: Path, dst: Path, ctime: Time)
+  requires PInv.Inv(fs)
+  requires PInv.Inv(fs')
+  requires P.Rename(fs, fs', src, dst, ctime)
+  requires dst != RootDir
+  requires I(fs').path_map == F.PathMapRename(I(fs), src, dst)
+  ensures I(fs').meta_map == F.MetaMapRename(I(fs), src, dst, ctime)
+  {
+    var i_fs := I(fs);
+    var i_fs' := I(fs');
+
+    var src_id := P.GetMeta(fs, src).id;
+    var src_m := P.GetMeta(fs, src);
+    var src_m' := P.MetaDataUpdateTime(src_m, src_m.atime, src_m.mtime, ctime);
+    assert src_id == i_fs.path_map[src] by { reveal_IPathMap(); }
+    GetMetaEquiv(fs, src);
+
+    var dst_id := if P.PathExists(fs, dst) then P.GetMeta(fs, dst).id else Nonexistent;
+    assert dst_id == i_fs.path_map[dst] by { reveal_IPathMap(); }
+    assert src_id == i_fs'.path_map[dst] by { reveal_IPathMap(); }
+
+    var src_parent_dir := GetParentDir(src);
+    var src_parent_id := P.GetMeta(fs, src_parent_dir).id;
+    assert src_parent_id == i_fs.path_map[src_parent_dir] by { reveal_IPathMap(); }
+    assert !BeneathDir(dst, src_parent_dir) by {
+       if BeneathDir(dst, src_parent_dir) {
+        PInv.NoValidBeneathDir(fs, dst, src_parent_dir);
+      }
+    }
+    GetMetaEquiv(fs, src_parent_dir);
+
+    var dst_parent_dir := GetParentDir(dst);
+    var dst_parent_id := P.GetMeta(fs, dst_parent_dir).id;
+    assert dst_parent_id == i_fs.path_map[dst_parent_dir] by { reveal_IPathMap(); }
+    GetMetaEquiv(fs, dst_parent_dir);
+
+    forall id
+    ensures i_fs'.meta_map[id] == F.MetaMapRename(i_fs, src, dst, ctime)[id]
+    {
+      if id == Nonexistent {
+        assert FInv.Inv(i_fs);
+        assert FInv.Inv(i_fs');
+      } else if id in i_fs.path_map.Values {
+        if id == src_id {
+          GetMetaEquiv(fs', dst);
+        } else if id == dst_id {
+          meow(fs, fs', src, dst, ctime);
+        } else if id == src_parent_id {
+          assert i_fs.path_map[src_parent_dir] == i_fs'.path_map[src_parent_dir];
+          GetMetaEquiv(fs', src_parent_dir);
+        } else if id == dst_parent_id {
+          assert i_fs.path_map[dst_parent_dir] == i_fs'.path_map[dst_parent_dir];
+          GetMetaEquiv(fs', dst_parent_dir);
+        } else {
+          assert exists p :: P.PathExists(fs, p) && P.GetMeta(fs, p).id == id by { reveal_IPathMap(); }
+          var p :| P.PathExists(fs, p) && P.GetMeta(fs, p).id == id;
+          if BeneathDir(dst, p) {
+            PInv.NoValidBeneathDir(fs, dst, p);
+            assert false;
+          } else if BeneathDir(src, p) {
+            var dstpath := dst + p[|src|..];
+            assert BeneathDir(dst, dstpath);
+            assert p == src + dstpath[|dst|..];
+            assert i_fs.path_map[p] == id by { reveal_IPathMap(); }
+            assert i_fs'.path_map[dstpath] == i_fs.path_map[p];
+            assert i_fs'.path_map[dstpath] == id;
+            GetMetaEquiv(fs, p);
+            GetMetaEquiv(fs', dstpath);
+          } else {
+            assert i_fs.path_map[p] == i_fs'.path_map[p];
+            assert i_fs.path_map[p] == id by { reveal_IPathMap(); }
+            assert P.GetMeta(fs, p) == P.GetMeta(fs', p);
+            GetMetaEquiv(fs, p);
+            GetMetaEquiv(fs', p);
+          }
+        }
+      } else {
+        assert id !in i_fs'.path_map.Values; // observe
+        reveal_IMetaMap();
+      }
+    }
+    Maps.IMapEquivalent(i_fs'.meta_map, F.MetaMapRename(i_fs, src, dst, ctime));
+  }
+
+  lemma RefinesRenameDataMap(fs: P.FileSys, fs': P.FileSys, src: Path, dst: Path, ctime: Time)
+  requires PInv.Inv(fs)
+  requires PInv.Inv(fs')
+  requires P.Rename(fs, fs', src, dst, ctime)
+  requires dst != RootDir
+  requires I(fs').path_map == F.PathMapRename(I(fs), src, dst)
+  requires I(fs').meta_map == F.MetaMapRename(I(fs), src, dst, ctime)
+  ensures I(fs').data_map == I(fs).data_map[I(fs).path_map[dst] := F.DataDelete(I(fs), dst)]
+  {
+    var i_fs := I(fs);
+    var i_fs' := I(fs');
+
+    var dst_id := if P.PathExists(fs, dst) then P.GetMeta(fs, dst).id else Nonexistent;
+    assert dst_id == i_fs.path_map[dst] by { reveal_IPathMap(); }
+
+    forall id
+    ensures i_fs'.data_map[id] == i_fs.data_map[dst_id := F.DataDelete(i_fs, dst)][id]
+    {
+      if id == Nonexistent {
+      }  else if id in i_fs.path_map.Values {
+        if id == dst_id {
+          meow(fs, fs', src, dst, ctime);
+        } else {
+          assert exists p :: P.PathExists(fs, p) && P.GetMeta(fs, p).id == id by { reveal_IPathMap(); }
+          var p :| P.PathExists(fs, p) && P.GetMeta(fs, p).id == id;
+          assert i_fs.path_map[p] == id by { reveal_IPathMap(); }
+
+          if p == src || BeneathDir(src, p) {
+            var dstpath := dst + p[|src|..];
+            assert p == src + dstpath[|dst|..];
+            assert i_fs'.path_map[dstpath] == i_fs.path_map[p];
+            assert i_fs'.path_map[dstpath] == id;
+            GetDataEquiv(fs, p);
+            GetDataEquiv(fs', dstpath);
+          } else if BeneathDir(dst, p) {
+            PInv.NoValidBeneathDir(fs, dst, p);
+          } else {
+            assert i_fs'.path_map[p] == i_fs.path_map[p];
+            GetDataEquiv(fs, p);
+            GetDataEquiv(fs', p);
+          }
+        }
+      } else {
+        assert id !in i_fs'.path_map.Values; // observe
+        assert i_fs.data_map[id] == EmptyData() by { reveal_IDataMap(); }
+        assert i_fs'.data_map[id] == EmptyData() by { reveal_IDataMap(); }
+      }
+    }
+    Maps.IMapEquivalent(i_fs'.data_map, i_fs.data_map[dst_id := F.DataDelete(i_fs, dst)]);
+  }
+
+  lemma {:timeLimitMultiplier 2} RefinesRename(fs: P.FileSys, fs': P.FileSys, src: Path, dst: Path, ctime: Time)
+  requires PInv.Inv(fs)
+  requires PInv.Inv(fs')
+  requires P.Rename(fs, fs', src, dst, ctime)
+  ensures F.Rename(I(fs), I(fs'), src, dst, ctime)
+  {
+    var i_fs := I(fs);
+    var i_fs' := I(fs');
+
+    if dst == RootDir {
+      PInv.NoValidBeneathDir(fs, dst, src);
+      assert false;
+    }
+
+    RefinesRenamePathMap(fs, fs', src, dst, ctime);
+    RefinesRenameMetaMap(fs, fs', src, dst, ctime);
+    RefinesRenameDataMap(fs, fs', src, dst, ctime);
+
+    reveal_IPathMap();
+    reveal_IMetaMap();
+    reveal_IDataMap();
+
+    assert F.Rename(i_fs, i_fs', src, dst, ctime);
   }
 
   lemma {:timeLimitMultiplier 3} RefinesLink(fs: P.FileSys, fs': P.FileSys, source: Path, dest: Path, ctime: Time, hiddenName: Option<Path>)
@@ -364,8 +674,8 @@ module PathBasedFSRefinement {
     ensures i_fs'.data_map[id] == i_fs.data_map[id]
     {
       if id == Nonexistent {
-        InvImpliesInv(fs);
-        InvImpliesInv(fs');
+        // InvImpliesInv(fs);
+        // InvImpliesInv(fs');
       } else if id in i_fs.path_map.Values {
         if id == src_id {
           if m.MetaData? {
@@ -447,7 +757,6 @@ module PathBasedFSRefinement {
   requires P.Write(fs, fs', path, offset, size, data, time)
   ensures F.Write(I(fs), I(fs'), path, offset, size, data, time)
   {
-    // TODO: fill in proof here
   }
 
   lemma RefinesUpdateTime(fs: P.FileSys, fs': P.FileSys, path: Path, atime: Time, mtime: Time, ctime: Time)
